Progress on FC for Blake2 incremental

code/blake2b/experimental/Hacl.Impl.Blake2b.Incremental.fst
@@ -30,14 +30,22 @@ noeq type state_r = {
 }
 
 
-let state_inv (h:mem) (state:state_r) =
+unfold let state_inv (h:mem) (state:state_r) =
   live h state.hash /\ live h state.block /\ disjoint state.hash state.block
 
-let state_empty (h:mem) (state:state_r) =
+unfold let state_empty (h:mem) (state:state_r) =
   h.[|state.hash|] == Lib.Sequence.create Spec.Blake2.size_hash_w (u64 0) /\
   v state.n == 0 /\
   v state.pl == 0 /\
   h.[|state.block|] == Lib.Sequence.create (Spec.Blake2.size_block Spec.Blake2.Blake2B) (u8 0)
+
+val state_hash_eq: h:mem -> state_r -> (Spec.state_r Spec.Blake2.Blake2B) -> prop
+let state_hash_eq h istate sstate =
+  sstate.Spec.hash == h.[|istate.hash|]
+
+val state_block_eq: h:mem -> state_r -> (Spec.state_r Spec.Blake2.Blake2B) -> prop
+let state_block_eq h istate sstate =
+  sstate.Spec.block == h.[|istate.block|]
 
 val state_eq: h:mem -> state_r -> (Spec.state_r Spec.Blake2.Blake2B) -> prop
 let state_eq h istate sstate =
@@ -45,6 +53,7 @@ let state_eq h istate sstate =
   sstate.Spec.n == v istate.n /\
   sstate.Spec.pl == v istate.pl /\
   sstate.Spec.block == h.[|istate.block|]
+
 
 val spec_of: h:mem -> state_r -> GTot (Spec.state_r Spec.Blake2.Blake2B)
 let spec_of h state =
@@ -64,24 +73,16 @@ val blake2b_incremental_init:
   (requires fun h ->
     live h state.hash /\ live h k /\
     disjoint state.hash k /\
+    state_inv h state /\
     state_empty h state)
   (ensures  fun h0 rstate h1 ->
     modifies1 state.hash h0 h1 /\
     spec_of h1 rstate == Spec.Blake2.Incremental.blake2_incremental_init Spec.Blake2.Blake2B h0.[|k|] (v nn))
 
 let blake2b_incremental_init state kk k nn =
-  (**) let h0 = ST.get () in
-  assert(state_empty h0 state);
-  assert(h0.[|state.block|] == Lib.Sequence.create (Spec.Blake2.size_block Spec.Blake2.Blake2B) (u8 0));
-  admit();
   blake2b_init state.hash kk k nn;
-  (**) let h1 = ST.get () in
-  [@inline_let]
   let n = if kk =. 0ul then 0ul else 1ul in
   let rstate = { state with n = n; } in
-  (**) let hf = ST.get () in
-  (**) assert(hf.[|rstate.hash|] == Spec.Blake2.blake2_init Spec.Blake2.Blake2B (v kk) h0.[|k|] (v nn));
-  (**) assert(hf.[|rstate.block|] == Seq.create (Spec.Blake2.size_block Spec.Blake2.Blake2B) (u8 0));
   rstate
 
 
